Refinement triple for write.

src/Examples/ReplicatedDisk/ReplicatedDiskImpl.v
@@ -6,13 +6,17 @@ From RecoveryRefinement Require Import TwoDiskAPI OneDiskAPI.
 Import TwoDisk.
 
 Definition write (addr: nat) (v: nat) :=
-  (_ <- lock addr;
+  (if lt_dec addr size then
+   _ <- lock addr;
    _ <- write_disk d0 addr v;
    _ <- write_disk d1 addr v;
-   unlock addr)%proc.
+   unlock addr
+   else (_ <- Ret tt; Ret tt))%proc.
+
 
 Definition read (addr: nat) :=
-  (_ <- lock addr;
+  (if lt_dec addr size then
+   _ <- lock addr;
    v <- (rd0 <- read_disk d0 addr;
            match rd0 with
            | Some v => Ret v
@@ -23,7 +27,8 @@ Definition read (addr: nat) :=
              end
            end);
    _ <- unlock addr;
-   Ret v)%proc.
+   Ret v
+   else (_ <- Ret tt; Ret 0))%proc.
 
 Definition fixup (a: addr) : proc Op unit :=
   (rd0 <- read_disk d0 a;
