src/Examples/ReplicatedDisk/ReplicatedDiskRefinement.v
@@ -1,0 +1,219 @@
+From iris.algebra Require Import auth gmap list.
+Require Export CSL.Refinement CSL.NamedDestruct.
+Require Import OneDiskAPI ReplicatedDiskImpl ReplicatedDisk.WeakestPre ReplicatedDisk.RefinementAdequacy.
+Set Default Proof Using "All".
+Unset Implicit Arguments.
+
+From Tactical Require Import UnfoldLemma.
+
+Definition gen_heap_ctx' {L V} `{Countable L} `{hG: gen_heapG L V Σ}
+  := (∃ σ, gen_heap_ctx σ)%I.
+Lemma gen_heap_update' {L V} `{Countable L} `{hG: gen_heapG L V Σ} l v1 v2:
+    gen_heap_ctx' -∗ mapsto l 1 v1 ==∗ gen_heap_ctx' ∗ mapsto l 1 v2.
+Proof.
+  iIntros "Hctx Hmapsto". iDestruct "Hctx" as (σ) "H".
+  iMod (gen_heap_update with "[$] [$]") as "(?&$)".
+  iExists _; eauto.
+Qed.
+
+Inductive addr_status :=
+| Sync
+| Unsync (j: nat) {T2} K `{LanguageCtx _ unit T2 OneDisk.l K}.
+
+Canonical Structure addr_statusC :=
+  leibnizC addr_status.
+Canonical Structure addr_statusF :=
+  discreteC addr_status.
+
+Section refinement_triples.
+  Context `{!exmachG Σ, lockG Σ, !@cfgG (OneDisk.Op) (OneDisk.l) Σ}.
+  Context {hD0Lease:  gen_heapG addr nat Σ}.
+  Context {hD1Lease:  gen_heapG addr nat Σ}.
+  Context {hSync: gen_heapG addr addr_status Σ}.
+
+  Notation "l l0↦{ q } v " := (mapsto (hG := hD0Lease) l q v)
+    (at level 20, q at level 50, format "l  l0↦{ q }  v") : bi_scope.
+  Notation "l l0↦ v " :=
+    (mapsto (hG := hD0Lease) l 1 v)
+    (at level 20) : bi_scope.
+  Notation "l l1↦{ q } v " := (mapsto (hG := hD1Lease) l q v)
+    (at level 20, q at level 50, format "l  l1↦{ q }  v ") : bi_scope.
+  Notation "l l1↦ v " :=
+    (mapsto (hG := hD1Lease) l 1 v)
+    (at level 20) : bi_scope.
+
+  Notation "l s↦{ q } v " := (mapsto (hG := hSync) l q v)
+    (at level 20, q at level 50, format "l  s↦{ q }  v") : bi_scope.
+
+  Definition LockInv (a: addr) :=
+    (∃ v, a l0↦{1/2} v ∗ a l1↦{1/2} v ∗ a s↦{1/2} Sync)%I.
+
+  Definition status_interp (a: addr) v0 v1 (s: addr_status) :=
+    (match s with
+     | Sync => ⌜ v0 = v1 ⌝
+     | Unsync j K => j ⤇ K (Call (OneDisk.Write_Disk a v0))
+     end)%I.
+
+  Global Instance status_interp_timeless a v0 v1 s:
+    Timeless (status_interp a v0 v1 s).
+  Proof. destruct s; apply _. Qed.
+
+  Definition DurInv (a: addr) v1 :=
+    (∃ v0 stat, a d0↦ v0 ∗ a d1↦ v1 ∗ a l0↦{1/2} v0 ∗ a l1↦{1/2} v1 ∗ a s↦{1/2} stat
+                  ∗ status_interp a v0 v1 stat)%I.
+
+  Definition durN : namespace := (nroot.@"dur_inv").
+  Definition lockN : namespace := (nroot.@"lock_inv").
+
+  Definition addrset := dom (gset nat) init_zero.
+  Opaque init_zero size.
+
+  Definition DisksInv :=
+    (∃ σ : OneDisk.State, ⌜ dom (gset _) (OneDisk.disk_state σ) = addrset ⌝ ∗ source_state σ
+       ∗ gen_heap_ctx' (hG := hD0Lease)
+       ∗ gen_heap_ctx' (hG := hD1Lease)
+       ∗ gen_heap_ctx' (hG := hSync)
+       ∗ [∗ map] a↦v1 ∈ OneDisk.disk_state σ, DurInv a v1)%I.
+
+  Definition ExecInv :=
+    (source_ctx ∗ ([∗ set] a ∈ addrset, ∃ γ, is_lock lockN γ a (LockInv a)) ∗ inv durN DisksInv)%I.
+
+  Global Instance addr_status_inhabited :
+    Inhabited (addr_status).
+  Proof. econstructor. exact Sync. Qed.
+
+  Global Instance odstate_inhaibted:
+    Inhabited (OneDisk.State).
+  Proof. econstructor. exact {| OneDisk.disk_state := init_zero |}. Qed.
+
+
+  Lemma not_lt_size_not_in_addrset a:
+    ¬ a < size → a ∉ addrset.
+  Proof. intros. apply not_elem_of_dom, init_zero_lookup_ge_None; lia. Qed.
+
+  Lemma lt_size_in_addrset a:
+    a < size → a ∈ addrset.
+  Proof. intros. apply elem_of_dom. eexists. apply init_zero_lookup_lt_zero; lia. Qed.
+
+  Opaque addrset.
+
+  Set Nested Proofs Allowed.
+  Lemma upd_disk_dom a v σ:
+    dom (gset nat) (OneDisk.upd_disk a v σ).(OneDisk.disk_state) =
+    dom (gset nat) σ.(OneDisk.disk_state).
+  Proof.
+    rewrite /OneDisk.upd_disk//=/OneDisk.upd_default//=.
+    destruct (_ !! a) as [?|] eqn:Hlookup.
+    - rewrite dom_insert_L.
+      assert (a ∈ dom (gset nat) σ.(OneDisk.disk_state)).
+      { apply elem_of_dom; eauto. }
+      set_solver.
+    - auto.
+  Qed.
+
+  Lemma write_refinement {T} j K `{LanguageCtx OneDisk.Op unit T OneDisk.l K} a v:
+    {{{ j ⤇ K (Call (OneDisk.Write_Disk a v)) ∗ Registered ∗ ExecInv }}}
+      write a v
+    {{{ v, RET v; j ⤇ K (Ret v) ∗ Registered }}}.
+  Proof.
+    iIntros (Φ) "(Hj&Hreg&(#Hsrc&#Hlocks&#Hinv)) HΦ".
+    rewrite /write. destruct lt_dec as [Hlt|Hnlt]; last first.
+    {
+      iApply wp_bind_proc_subst.
+      iInv "Hinv" as "H".
+      iDestruct "H" as (σ) "(>Hdom1&>Hstate&?)".
+      iDestruct "Hdom1" as %Hdom1.
+      iMod (ghost_step_call with "Hj Hsrc [$]") as "(Hj&Hstate&_)".
+      { intros. do 2 eexists; split; last econstructor.
+        split; auto.
+        econstructor.
+      }
+      { solve_ndisj. }
+      wp_ret.
+      assert ((OneDisk.upd_disk a v σ) = σ) as ->.
+      {  destruct σ as [d].
+         rewrite /OneDisk.upd_disk. f_equal.
+         rewrite /OneDisk.upd_default.
+         pose proof (not_lt_size_not_in_addrset a Hnlt) as Hdom.
+         rewrite -Hdom1 not_elem_of_dom in Hdom * => ->.
+         eauto.
+      }
+      iExists _. iFrame. iSplitL "".
+      { iModIntro. iNext. iPureIntro. auto. }
+      iModIntro. iNext. wp_ret. clear. iApply "HΦ". iFrame.
+    }
+    wp_bind. apply lt_size_in_addrset in Hlt.
+    iDestruct (big_sepS_elem_of with "Hlocks") as "Hlock"; first eauto.
+    iDestruct "Hlock" as (γ) "Hlock".
+    iApply (wp_lock with "[$]").
+    iIntros "!> (Hlocked&Hlockinv)".
+    wp_bind. iDestruct "Hlockinv" as (v') "(Hl0&Hl1&Hstatus)".
+    iInv "Hinv" as "H".
+    iDestruct "H" as (σ) "(>Hdom1&>Hstate&Hctx0&Hctx1&Hctx_stat&>Hdur)".
+    iDestruct "Hdom1" as %Hdom1.
+    generalize Hlt => Hdom2.
+    rewrite -Hdom1 in Hdom2.
+    rewrite elem_of_dom in Hdom2 *. intros [v1 Hlookup].
+    iDestruct (big_sepM_lookup_acc with "Hdur") as "(Hcurr&Hdur)"; first eauto.
+    iDestruct "Hcurr" as (v0 stat) "(Hd0&Hd1&Hl0_auth&Hl1_auth&Hstatus_auth&Hstat)".
+    iDestruct (mapsto_agree with "Hl0 Hl0_auth") as %Heq; subst.
+    iDestruct (mapsto_agree with "Hl1 Hl1_auth") as %Heq; subst.
+    iDestruct (mapsto_agree with "Hstatus Hstatus_auth") as %Heq; subst.
+    iDestruct "Hstat" as %Heq; subst.
+    iApply (wp_write_disk0 with "[$]").
+    iIntros "!> Hd0".
+    iMod (gen_heap_update' _ _ v with "Hctx0 [Hl0 Hl0_auth]") as "(?&Hl0)".
+    { iCombine "Hl0 Hl0_auth" as "$". }
+    iDestruct "Hl0" as "(Hl0&Hl0_auth)".
+    iMod (gen_heap_update' _ _ (Unsync j K) with "[$] [Hstatus Hstatus_auth]") as "(?&Hstatus)".
+    { iCombine "Hstatus Hstatus_auth" as "$". }
+    iDestruct "Hstatus" as "(Hstatus&Hstatus_auth)".
+    iExists _. iFrame.
+    iSplitL "Hdur Hd0 Hd1 Hl0_auth Hl1_auth Hstatus_auth Hj".
+    { iSplitL ""; first by iPureIntro.
+      iApply "Hdur". iExists _, _. iFrame.
+      iFrame. clear. iClear "Hlocks". auto. }
+    iModIntro. wp_bind.
+
+    iInv "Hinv" as "H".
+    clear σ Hdom1 Hlookup Heq.
+    iDestruct "H" as (σ) "(>Hdom1&>Hstate&Hctx0&Hctx1&Hctx_stat&>Hdur)".
+    iDestruct "Hdom1" as %Hdom1.
+    generalize Hlt => Hdom2.
+    rewrite -Hdom1 in Hdom2.
+    rewrite elem_of_dom in Hdom2 *. intros [v1' Hlookup].
+    iDestruct (big_sepM_insert_acc with "Hdur") as "(Hcurr&Hdur)"; first eauto.
+    iDestruct "Hcurr" as (? ?) "(Hd0&Hd1&Hl0_auth&Hl1_auth&Hstatus_auth&Hstat)".
+    iDestruct (mapsto_agree with "Hl0 Hl0_auth") as %<-; subst.
+    iDestruct (mapsto_agree with "Hl1 Hl1_auth") as %Heq; subst.
+    iDestruct (mapsto_agree with "Hstatus Hstatus_auth") as %Heq; subst.
+    iApply (wp_write_disk1 with "[$]").
+    iIntros "!> Hd1".
+    iMod (gen_heap_update' _ _ v with "[$] [Hl1 Hl1_auth]") as "(?&Hl1)".
+    { iCombine "Hl1 Hl1_auth" as "$". }
+    iDestruct "Hl1" as "(Hl1&Hl1_auth)".
+    iMod (gen_heap_update' _ _ Sync with "[$] [Hstatus Hstatus_auth]") as "(?&Hstatus)".
+    { iCombine "Hstatus Hstatus_auth" as "$". }
+    iDestruct "Hstatus" as "(Hstatus&Hstatus_auth)".
+    iMod (ghost_step_call with "Hstat Hsrc [$]") as "(Hj&Hstate&_)".
+    { intros. do 2 eexists; split; last econstructor.
+      split; auto.
+      econstructor.
+    }
+    { solve_ndisj. }
+    iExists _. iFrame.
+
+    rewrite upd_disk_dom.
+    iSplitL "Hdur Hd0 Hd1 Hl0_auth Hl1_auth Hstatus_auth".
+    { iSplitL ""; first by iPureIntro.
+      iModIntro. iNext.
+      rewrite /OneDisk.upd_disk/OneDisk.upd_default /= Hlookup.
+      iApply "Hdur". iExists _, _. iFrame.
+      iFrame. clear. iClear "Hlocks". auto. }
+
+    iApply (wp_unlock with "[Hl0 Hl1 Hstatus Hlocked]").
+    { iFrame "Hlock". iFrame. iExists _; iFrame. }
+    iIntros "!> _". iApply "HΦ". iFrame.
+  Qed.
+
+End refinement_triples.
